multiset/progStepImpliesSpec.v
@@ -1,6 +1,9 @@
 Require Import erasure.  
 Require Import NonSpecPureStep. 
 Require Import eraseRollbackIdempotent. 
+Require Import IndependenceCommon.
+Require Import SpecImpliesNonSpec.
+Require Import progStepWF. 
 
 (*H; T ->+ H'; T'*)
 Inductive pstepPlus : pHeap -> pPool -> pHeap -> pPool -> Prop :=
@@ -32,7 +35,7 @@ Theorem lookupEraseCommitEmpty : forall x H,
 Proof.
   intros. destruct H. simpl. eapply raw_lookupEraseCommitEmpty; eauto. 
 Qed. 
-
+ 
 Theorem raw_eraseCommitWrite : forall x H ds TID N, 
                              raw_heap_lookup x H = Some (sempty COMMIT) ->
                              raw_eraseHeap (raw_replace x (sfull COMMIT ds COMMIT TID N) H) = 
@@ -54,96 +57,65 @@ Theorem eraseCommitWrite : forall x H ds TID N,
                              replace x (pfull (eraseTerm N)) (eraseHeap H). 
 Proof.
   intros. destruct H. simpl. apply rawHeapsEq. eapply raw_eraseCommitWrite; eauto.
+Qed.
+
+Theorem unspecEmpty : forall tid s2 M s1, 
+                        unspecPool(tSingleton(tid,locked s1, s2, M)) = 
+                        Empty_set thread. auto. Qed. 
+
+Theorem raw_lookupEraseNoneNone : forall x H, 
+                                raw_heap_lookup x H = None ->
+                                raw_heap_lookup x (raw_eraseHeap H) = None. 
+Proof.
+  induction H; intros. 
+  {auto. }
+  {simpl in *. destruct a. destruct (beq_nat x i) eqn:eq. 
+   {inv H0. }
+   {destruct i0. destruct s; auto. simpl. rewrite eq; auto. 
+    destruct s; auto. destruct s0; simpl; rewrite eq; auto. }
+  }
 Qed. 
 
-Theorem specImpliesNonSpec : forall H H' T t t', 
+Theorem lookupEraseNoneNone : forall x H, 
+                                heap_lookup x H = None ->
+                                heap_lookup x (eraseHeap H) = None. 
+Proof.
+  intros. destruct H. simpl. eapply raw_lookupEraseNoneNone; eauto. 
+Qed. 
+
+Theorem prog_specImpliesNonSpec : forall H H' T t t', 
                                prog_step H T t (OK H' T t') -> wellFormed H (tUnion T t) ->
                                exists PH' T', pstepPlus (eraseHeap H) (erasePool (tUnion T t)) PH' T' /\
                                                eraseHeap H' = PH' /\ erasePool (tUnion T t') = T'. 
 Proof.
   intros. inv H0. 
   {exists (eraseHeap H'). econstructor. split; auto. repeat rewrite eraseUnionComm. 
-   simpl. apply simBasicStep in H6. econstructor. eapply PBasicStep. eauto. constructor. }
-  {exists (eraseHeap H'). econstructor. split; auto. unfoldTac. rewrite coupleUnion. 
-   repeat rewrite eraseUnionComm. simpl. copy d. erewrite <- decomposeErase in H; eauto.
-   econstructor. eapply pFork. eauto. rewrite eraseFill. constructor. }
-  {copy d. erewrite <- decomposeErase in H0; eauto. econstructor. econstructor. 
-   split. rewrite eraseUnionComm. simpl. econstructor. eapply PGet; eauto.
-   eapply lookupEraseCommitFull; eauto. eassumption. constructor. split.
-   erewrite eraseHeapDependentRead; eauto. rewrite eraseUnionComm. simpl. 
-   rewrite eraseFill. auto. }
-  {erewrite <- decomposeErase in H4; eauto. econstructor. econstructor. split. 
-   rewrite eraseUnionComm. simpl. econstructor. eapply PPut. simpl in *. eauto.
-   eapply lookupEraseCommitEmpty; eauto. auto. constructor. split. 
-   apply eraseCommitWrite; eauto. rewrite eraseUnionComm. simpl. rewrite eraseFill; auto. }
+   simpl. apply simBasicStep in H6. econstructor. eapply PBasicStep. eauto. 
+   constructor. }
   {apply rollbackIdempotent in H7. invertHyp. copy d.
    erewrite <- decomposeErase in H3; eauto. econstructor. econstructor. split. 
    unfoldTac. rewrite AddUnion. rewrite Union_associative. rewrite eraseUnionComm.
    econstructor. eapply PPut. simpl in *. copy H3. apply pdecomposeEq in H3. 
    rewrite H3 in H7. rewrite eraseFill; eauto. eapply lookupEraseSpecFull; eauto. 
-   auto. constructor. split. apply eraseHeapCommitWrite. 
-
-
-
-inv H1. destruct s1. 
-   {simpl. constructor. }
-   {destructLast l. 
-    {simpl. constructor. }
-    {invertHyp. unfoldTac. rewrite coupleUnion. rewrite eraseUnionComm. actTermTac x. 
-     erewrite eraseLastAct; eauto. rewrite eraseEmpty. unfold pUnion.
-     rewrite union_empty_r. erewrite eraseTwoActs'; eauto. constructor. }
-   }
-   {simpl. constructor. }
-  }
-  {exists (eraseHeap H). destruct s1. 
-   {econstructor. split. simpl. constructor. erewrite eraseHeapDependentRead; eauto. }
-   {destructLast l. 
-    {econstructor. split. simpl. constructor. erewrite eraseHeapDependentRead; eauto. }
-    {invertHyp. econstructor. split. constructor. split. erewrite eraseHeapDependentRead; eauto. 
-     inv H1. actTermTac x0. erewrite eraseTwoActs'; eauto. erewrite eraseLastAct; eauto. }
-   }
-   {econstructor. split. simpl. constructor. erewrite eraseHeapDependentRead; eauto. }
-  }
-  {exists (eraseHeap H). econstructor. split. constructor. split. erewrite eraseHeapWrite; auto.
-   inv H1. destruct s1; auto. 
-   {destructLast l; auto. invertHyp. actTermTac x0. erewrite eraseTwoActs'; eauto. 
-    erewrite eraseLastAct; eauto. }
-  }  
-  {exists (eraseHeap H). eapply rollbackIdempotent in H7; eauto. 
-   invertHyp. inv H1. econstructor. split. constructor. split. 
-   erewrite eraseHeapWrite; auto. unfoldTac. repeat rewrite AddUnion. 
-   repeat rewrite eraseUnionComm. rewrite <- H0. simpl. apply decomposeEq in d. 
-   subst. auto. }
-  {exists (eraseHeap H). econstructor. split. constructor. split. 
-   rewrite eraseHeapNew. auto. inv H1. destruct s1; auto. 
-   {destructLast l. 
-    {copy d. apply decomposeEq in H0. subst. simpl. auto. }
-    {invertHyp. actTermTac x0. erewrite eraseTwoActs'; eauto. erewrite eraseLastAct; eauto. }
-   }
-  }
-  {exists (eraseHeap H'). econstructor. split; auto. inv H1. unfoldTac. rewrite coupleUnion. 
-   rewrite eraseUnionComm. destruct s1.
-   {simpl. constructor. }
-   {destructLast l. 
-    {simpl. constructor. }
-    {invertHyp. actTermTac x. erewrite eraseLastAct; eauto.
-     erewrite eraseTwoActs'; eauto. simpl. constructor. }
-   }
-   {simpl. constructor. }
-  }
+   auto. constructor. split. rewrite H2. eapply eraseCommitWrite; eauto. 
+   unfoldTac. rewrite AddUnion. rewrite Union_associative. rewrite eraseUnionComm. 
+   simpl. rewrite eraseFill; eauto. repeat rewrite eraseUnionComm. rewrite H0. 
+   auto. }
   {inv H1. unfoldTac. rewrite coupleUnion in H0. 
    repeat rewrite unspecUnionComm in H0. econstructor. econstructor. split; auto. 
-   rewrite coupleUnion. rewrite eraseUnionComm. rewrite eraseEmptySpec. unfold pUnion. 
-   rewrite union_empty_r. repeat rewrite Union_associative in H0. econstructor. 
-   eapply pSpecRun. copy p. erewrite <- decomposeErase in H; eauto. simpl. auto. 
-   copy p. apply decomposeWF in H. rewrite eraseCtxtWF in H. simpl in H. copy p. 
-   rewrite <- decomposeErase in H1; eauto. simpl in H1. destructLast s1. 
+   rewrite coupleUnion. repeat rewrite eraseUnionComm. rewrite eraseEmptySpec. 
+   unfold pUnion. rewrite union_empty_r. repeat rewrite Union_associative in H0. 
+   econstructor. eapply pSpecRun. copy p. erewrite <- decomposeErase in H; eauto. 
+   simpl. auto. copy p. apply decomposeWF in H. rewrite eraseCtxtWF in H. 
+   simpl in H. copy p. rewrite <- decomposeErase in H1; eauto. simpl in H1. 
+   destructLast s1. 
    {simpl. rewrite eraseFill. unfoldTac. rewrite UnionSwap in H0.
     rewrite Union_associative in H0. rewrite UnionSwap in H0.
     rewrite spec_multi_unused in H0. eapply simSpecJoinSteps; eauto. simpl in *.
     eassumption. }
-   {unfoldTac. rewrite UnionSwap in H0. rewrite Union_associative in H0. rewrite UnionSwap in H0. 
-    rewrite spec_multi_unused in H0. invertHyp. rewrite wrapDistributeApp. destruct x.
+   {unfoldTac. rewrite UnionSwap in H0. rewrite Union_associative in H0. 
+    rewrite UnionSwap in H0. rewrite spec_multi_unused in H0. invertHyp. 
+    rewrite wrapDistributeApp. destruct x.
     {simpl (wrapActs [rAct x t E0 d] N1 E (specRun (ret N1) N0)(decomposeWF t0 E (specRun (ret N1) N0) p)).
      erewrite eraseLastAct; eauto. eauto. rewrite eraseFill. 
      eapply simSpecJoinSteps';[idtac|eauto|simpl in *; eauto]. constructor. }
@@ -161,51 +133,58 @@ inv H1. destruct s1.
      eapply simSpecJoinSteps'; [idtac|eauto|simpl in *; eauto]. constructor. }
    }
   }
-  {exists (eraseHeap H). eapply rollbackIdempotent in H10; eauto. 
-   invertHyp. inv H1. econstructor. split. unfoldTac. rewrite coupleUnion. 
-   repeat rewrite eraseUnionComm. unfold pUnion. rewrite Union_associative. eapply pmulti_step. 
-   simpl. eapply pSpecRunRaise. eapply decomposeErase in H4; eauto. simpl. auto. 
-   unfold pUnion.  rewrite <- Union_associative. 
-   constructor. split; auto. unfoldTac. rewrite AddUnion. rewrite eraseUnionComm. 
-   repeat rewrite AddUnion in H0. repeat rewrite eraseUnionComm in H0. simpl in H0. 
-   unfold pUnion in H0. repeat rewrite union_empty_r in H0. rewrite <- H0.
-   simpl. rewrite eraseFill; eauto. }
+  {apply rollbackIdempotent in H10. invertHyp.
+   erewrite <- decomposeErase in H4; eauto. econstructor. econstructor. split. 
+   unfoldTac. rewrite Union_associative. rewrite coupleUnion. 
+   repeat rewrite eraseUnionComm. simpl. econstructor. eapply pSpecRunRaise. 
+   simpl in *; eauto. constructor. split. auto. unfoldTac. rewrite AddUnion. 
+   rewrite Union_associative. repeat rewrite eraseUnionComm. simpl. 
+   repeat rewrite AddUnion in H0. rewrite Union_commutative in H0. simpl in H0. 
+   rewrite Union_commutative in H0. simpl in H0. rewrite H0.
+   rewrite eraseFill; eauto. }
   {exists (eraseHeap H). econstructor. split. Focus 2. split; auto. 
    erewrite eraseHeapDependentRead. auto. eauto. inv H1. eraseTrmTac s1' M. 
-   erewrite eraseLastAct; eauto. econstructor. eapply PGet; eauto. 
-   eapply lookupEraseCommitFull; eauto. copy d. erewrite <- decomposeErase in H0; eauto. 
-   rewrite unspecUnionComm in H2. erewrite unspecLastActPool in H2. Focus 2. constructor. 
+   rewrite eraseUnionComm. erewrite eraseLastAct; eauto. econstructor. 
+   eapply PGet; eauto. eapply lookupEraseCommitFull; eauto. copy d. 
+   erewrite <- decomposeErase in H0; eauto. rewrite unspecUnionComm in H2. 
+   erewrite unspecLastActPool in H2. Focus 2. constructor. 
    eapply specStepRead in H2; eauto. invertHyp. eapply simPureSteps in H0; eauto.
-   rewrite eraseFill in H0. simpl in H0. erewrite eraseEraseTrm; eauto. 
-   eapply unspecHeapLookupFull; eauto. }
+   rewrite eraseFill in H0. simpl in H0. rewrite eraseUnionComm. 
+   erewrite eraseEraseTrm; eauto. eapply unspecHeapLookupFull; eauto. }
   {exists (replace x (pfull (eraseTerm M'')) (eraseHeap H)). econstructor. split. 
    Focus 2. split; eauto. erewrite eraseHeapCommitWrite; eauto. inv H1. 
-   erewrite eraseLastAct. Focus 2. constructor. rewrite unspecUnionComm in H2. 
-   erewrite unspecLastActPool in H2. Focus 2. constructor. eraseTrmTac s1' M. 
-   erewrite eraseEraseTrm; eauto. eapply specStepWrite in H2; eauto. invertHyp. 
-   eapply simPureSteps in H0; eauto. rewrite eraseFill in H0. simpl in H0. 
-   econstructor. eapply PPut; eauto. copy d. erewrite <- decomposeErase in H2; eauto.
-   simpl. auto. eapply lookupEraseSpecFull; eauto. eassumption. 
+   repeat rewrite eraseUnionComm. erewrite eraseLastAct. Focus 2. constructor. 
+   rewrite unspecUnionComm in H2. erewrite unspecLastActPool in H2. Focus 2. 
+   constructor. eraseTrmTac s1' M. erewrite eraseEraseTrm; eauto.
+   eapply specStepWrite in H2; eauto. invertHyp. eapply simPureSteps in H0; eauto. 
+   rewrite eraseFill in H0. simpl in H0. econstructor. eapply PPut; eauto. copy d. 
+   erewrite <- decomposeErase in H2; eauto. simpl. auto. 
+   eapply lookupEraseSpecFull; eauto. eassumption.
    eapply lookupUnspecSpecFullEmpty; eauto. }
   {inv H1. assert(heap_lookup i (eraseHeap H) = None). 
    eapply lookupEraseSpecNone; eauto. exists (Heap.extend i pempty (eraseHeap H) H0). 
    econstructor. split. Focus 2. split; eauto. eapply eraseHeapCommitNewFull; eauto. 
-   erewrite eraseLastAct. Focus 2. constructor. econstructor.
-   eapply PNew with(x:=i)(p:=H0); eauto. copy d. erewrite <- decomposeErase in H1; eauto. 
-   rewrite unspecUnionComm in H2. erewrite unspecLastActPool in H2. Focus 2. constructor. 
-   eraseTrmTac s1' M. eapply specStepNewFull in H2; eauto. invertHyp. 
-   eapply simPureSteps in H1; eauto. rewrite eraseFill in H1.
-   erewrite eraseEraseTrm; eauto. eapply lookupUnspecSpecNone; eauto. }
-  {inv H1. assert(heap_lookup i (eraseHeap H) = None). eapply lookupEraseSpecNoneEmpty; eauto. 
-   exists (Heap.extend i pempty (eraseHeap H) H0). econstructor. split. Focus 2. split; eauto. 
-   eapply eraseHeapCommitNewEmpty; eauto. erewrite eraseLastAct. Focus 2. constructor. 
-   econstructor. eapply PNew with (x:=i)(p:=H0); eauto. copy d.
-   erewrite <- decomposeErase in H1; eauto. eraseTrmTac s1' M. erewrite eraseEraseTrm; eauto. 
-   rewrite unspecUnionComm in H2. erewrite unspecLastActPool in H2. Focus 2. constructor. 
-   eapply specStepNewEmpty in H2; eauto. invertHyp. eapply simPureSteps in H1; eauto. 
-   rewrite eraseFill in H1. eassumption. eapply lookupUnspecSpecEmptyNone; eauto. }
+   repeat rewrite eraseUnionComm. erewrite eraseLastAct. Focus 2. constructor. 
+   econstructor. eapply PNew with(x:=i)(p:=H0); eauto. copy d. 
+   erewrite <- decomposeErase in H1; eauto. rewrite unspecUnionComm in H2. 
+   erewrite unspecLastActPool in H2. Focus 2. constructor. eraseTrmTac s1' M. 
+   eapply specStepNewFull in H2; eauto. invertHyp. eapply simPureSteps in H1; eauto.
+   rewrite eraseFill in H1. erewrite eraseEraseTrm; eauto. 
+   eapply lookupUnspecSpecNone; eauto. }
+  {inv H1. assert(heap_lookup i (eraseHeap H) = None). 
+   eapply lookupEraseSpecNoneEmpty; eauto. 
+   exists (Heap.extend i pempty (eraseHeap H) H0). econstructor. split. Focus 2. 
+   split;eauto. eapply eraseHeapCommitNewEmpty; eauto. repeat rewrite eraseUnionComm.
+   erewrite eraseLastAct. Focus 2. constructor. econstructor. 
+   eapply PNew with (x:=i)(p:=H0); eauto. copy d.
+   erewrite <- decomposeErase in H1; eauto. eraseTrmTac s1' M.
+   erewrite eraseEraseTrm; eauto. rewrite unspecUnionComm in H2. 
+   erewrite unspecLastActPool in H2. Focus 2. constructor.
+   eapply specStepNewEmpty in H2; eauto. invertHyp.
+   eapply simPureSteps in H1; eauto. rewrite eraseFill in H1. eassumption. 
+   eapply lookupUnspecSpecEmptyNone; eauto. }
   {exists (eraseHeap H'). econstructor. split; auto. inv H1.
-   unfoldTac. rewrite coupleUnion. rewrite eraseUnionComm. rewrite eraseEmpty. 
+   unfoldTac. rewrite coupleUnion. repeat rewrite eraseUnionComm. rewrite eraseEmpty. 
    unfold pUnion. rewrite union_empty_r. erewrite eraseLastAct. Focus 2. constructor. 
    econstructor. eapply pFork. copy d. erewrite <- decomposeErase in H; eauto. 
    simpl. auto. rewrite coupleUnion in H0. repeat rewrite unspecUnionComm in H0. 
@@ -215,7 +194,7 @@ inv H1. destruct s1.
    rewrite <- H1. eraseTrmTac s1' M. eraseTrmTac s1'' N. unfoldTac.
    repeat rewrite coupleUnion in H. repeat rewrite Union_associative in H. 
    repeat rewrite coupleUnion. rewrite eraseUnionComm.
-   repeat erewrite eraseEraseTrm; eauto. unfold pUnion. repeat rewrite <- coupleUnion. 
+   repeat erewrite eraseEraseTrm;eauto. unfold pUnion. repeat rewrite <- coupleUnion. 
    copy H. eapply simPureStepsCouple' with(H'':=eraseHeap x)(PT:=erasePool T)
     (N:=pfill (eraseCtxt E)(pret punit)) in H; eauto. unfold pCouple. rewrite couple_swap. 
    eapply pmulti_trans. eassumption. rewrite UnionSwap in H0. rewrite <- Union_associative in H0. 
@@ -235,18 +214,6 @@ inv H1. destruct s1.
    eapply simPureSteps in H; eauto. rewrite eraseFill in H. eassumption. }
 Qed. 
 
-Theorem specImpliesNonSpecMulti : forall H H' T T', 
-                multistep H T (Some(H', T')) -> wellFormed H T -> 
-                exists PH' PT', pmultistep (eraseHeap H) (erasePool T) (Some(PH',PT')) /\
-                                eraseHeap H' = PH' /\ erasePool T' = PT'. 
-Proof.  
-  intros. depInd H0; intros.  
-  {econstructor. econstructor. split. constructor. auto. }
-  {copy H0. eapply specImpliesNonSpec in H0; eauto. invertHyp.
-   copy H3. eapply stepWF in H3; auto. eapply IHmultistep in H3; eauto. 
-   invertHyp. econstructor. econstructor. split; eauto. eapply pmulti_trans.
-   rewrite eraseUnionComm. eassumption. rewrite <- eraseUnionComm. auto. }
-Qed. 
 
 
 
@@ -254,6 +221,3 @@ Qed.
 
 
 
-
-
-asdlkfjhalsdkjfh
